Port basic concurrent cache definitions
State the AsyncRead spec (the lowest-level helper function) in terms of
new linearizable spec style. Without notation it's a bit awkward, but
seems to say what we want.

src/ConcurrentCache2.v
@@ -1,11 +1,15 @@
 Require Import EventCSL.
 Require Import EventCSLauto.
 Require Import Locking.
+Require Import HlistMem.
 Require Import Preservation.
 Require Import MemCache2.
 Require Import Automation.
 Require Import Locks.
 Require Import Linearizable.
+Require Import RelationCombinators.
+Require Import Omega.
+Import HlistNotations.
 
 Import List.
 Import List.ListNotations.
@@ -81,26 +85,225 @@ Module Type CacheSemantics (Sem:Semantics) (CVars:CacheVars Sem).
     Inv m s d ->
     cacheI m s d.
 
-  Axiom cache_relation_holds : forall s s' tid,
-      R tid s s' ->
-      cacheR tid s s'.
+  Axiom cache_relation_holds : forall tid,
+      rimpl (R tid) (cacheR tid).
 
   (* Here need to incorporate linearizability in order to say
   something powerful enough that specs can export Inv/R but can still
   freely modify variables in critical sections. *)
 
   Axiom cache_invariant_preserved : forall m s d m' s' d',
-    Inv m s d ->
-    cacheI m' s' d' ->
-    (* only memVars/stateVars were modified *)
-    modified memVars m m' ->
-    modified stateVars s s' ->
-    Inv m' s' d'.
+      Inv m s d ->
+      cacheI m' s' d' ->
+      modified memVars m m' ->
+      (* GDisk0 may not be modified, so the global invariant can state
+    interactions between the linearized disk and the rest of the ghost
+    state, which must be proven after unlocking. *)
+      modified [( GDisk; GCache; GLocks )] s s' ->
+      Inv m' s' d'.
 
-  Axiom cache_relation_preserved : forall tid s s' s'',
-    R tid s s' ->
-    modified stateVars s' s'' ->
-    cacheR tid s' s'' ->
-    R tid s s''.
+  Axiom cache_relation_preserved : forall tid s s',
+      (* can actually also assume anything about s that Inv m s d
+      implies (forall m and d) *)
+      modified [( GDisk; GCache; GLocks )] s s' ->
+      cacheR tid s s' ->
+      R tid s s'.
 
 End CacheSemantics.
+
+Module Cache (Sem:Semantics)
+  (CVars:CacheVars Sem)
+  (CSem:CacheSemantics Sem CVars).
+
+Import CSem.
+Import Sem.
+Import CVars.
+Import Transitions.
+
+Definition M := EventCSL.M Mcontents.
+Definition S := EventCSL.S Scontents.
+
+Lemma others_cache_relation_holds : forall tid,
+    rimpl (othersR R tid) (othersR cacheR tid).
+Proof.
+  unfold rimpl, othersR; intros.
+  deex.
+  eexists; intuition eauto.
+  apply cache_relation_holds; auto.
+Qed.
+
+Ltac derive_local_relations :=
+  repeat match goal with
+         | [ H: star R _ _ |- _ ] =>
+            learn H (rewrite cache_relation_holds in H)
+         | [ H: star (othersR R _) _ _ |- _ ] =>
+            learn H (rewrite others_cache_relation_holds in H)
+         end.
+
+Definition stateS : transitions Mcontents Scontents :=
+  Build_transitions R Inv.
+
+Ltac vars_distinct :=
+  repeat rewrite member_index_eq_var_index;
+  repeat match goal with
+  | [ |- context[var_index ?v] ] => unfold v
+  end;
+  repeat erewrite get_hmap; cbn;
+  apply NoDup_get_neq with (def := 0); eauto;
+    autorewrite with hlist;
+    cbn;
+    match goal with
+    | [ |- _ < _ ] => omega
+    | [ |- NoDup _ ] =>
+      apply no_confusion_memVars ||
+            apply no_confusion_stateVars
+    end.
+
+Ltac distinct_pf var1 var2 :=
+  assert (member_index var1 <> member_index var2) as Hneq
+    by vars_distinct;
+  exact Hneq.
+
+Hint Immediate
+     (ltac:(distinct_pf MLocks Cache)).
+
+Hint Immediate
+     (ltac:(distinct_pf GDisk GDisk0))
+     (ltac:(distinct_pf GDisk GCache))
+     (ltac:(distinct_pf GDisk GLocks))
+     (ltac:(distinct_pf GDisk0 GCache))
+     (ltac:(distinct_pf GDisk0 GLocks))
+     (ltac:(distinct_pf GCache GLocks)).
+
+Hint Resolve not_eq_sym.
+
+(*
+
+TODO: maybe copy over the proofs that simplify othersR cacheR
+(although cacheR now has almost nothing, since lock_protects seems to
+be implemented by the linearized consistency invariant).
+
+*)
+
+Ltac descend :=
+  match goal with
+  | [ |- forall _, _ ] => intros
+  | [ |- _ /\ _ ] => split
+  end.
+
+Ltac destruct_cache_entry :=
+  match goal with
+  | [ cache_entry: bool * valu |- _ ] =>
+    destruct cache_entry as [ [] ]
+  end.
+
+Ltac simplify_reduce_step :=
+  (* this binding just fixes PG indentation *)
+  let unf := autounfold with prog in * in
+          deex_local
+          || destruct_ands
+          || destruct_cache_entry
+          || descend
+          || subst
+          || unf.
+
+Ltac simplify_step :=
+    (time "simplify_reduce" simplify_reduce_step).
+
+Ltac simplify' t :=
+  repeat (repeat t;
+    repeat lazymatch goal with
+    | [ |- exists _, _ ] => eexists
+    end);
+  cleanup.
+
+Ltac simplify := simplify' simplify_step.
+
+Ltac solve_global_transitions :=
+  (* match only these types of goals *)
+  lazymatch goal with
+  | [ |- R _ _ _ ] =>
+    eapply cache_relation_preserved
+  | [ |- Inv _ _ _ ] =>
+    eapply cache_invariant_preserved
+  end.
+
+Hint Unfold GCache GDisk GDisk0 Cache : modified.
+Hint Resolve modified_nothing one_more_modified modified_single_var : modified.
+Hint Constructors HIn : modified.
+
+Ltac solve_modified :=
+  solve [ autounfold with modified; eauto with modified ].
+
+Ltac finish :=
+  try time "finisher" progress (
+  try time "solve_global_transitions" solve_global_transitions;
+  try time "congruence" (unfold wr_set, const in *; congruence);
+  try time "finish eauto" solve [ eauto ];
+  try time "solve_modified" solve_modified;
+  try time "pred_solve" solve [ pred_apply; cancel ]).
+
+Definition locked_AsyncRead {T} a rx : prog Mcontents Scontents T :=
+  tid <- GetTID;
+  GhostUpdate (fun s =>
+                 let vd := get GDisk s in
+                 let vd' := match vd (a, Owned tid) with
+                            | Some (vs, _) => upd vd (a, Owned tid) (vs, Some tid)
+                            (* impossible, cannot read if sector does
+                            not exist *)
+                            | None => vd
+                            end in
+                 set GDisk vd' s);;
+              StartRead a;;
+              Yield a;;
+              v <- FinishRead a;
+  GhostUpdate (fun s =>
+                 let vd := get GDisk s in
+                 let vd' := match vd (a, Owned tid) with
+                            | Some (vs, _) => upd vd (a, Owned tid) (vs, None)
+                            (* impossible, cannot read if sector does
+                            not exist *)
+                            | None => vd
+                            end in
+                 set GDisk vd' s);;
+              rx v.
+
+Definition cache_locked tid s (F: DISK_PRED) : DISK_PRED :=
+  locks_held (fun (s:S) (a:addr) => Locks.get (get GLocks s) a = Owned tid) s F.
+
+Theorem locked_AsyncRead_ok : forall a,
+  stateS TID: tid |-
+  {{ Fs Fs' F LF F' v vd,
+   | PRE d m s0 s:
+       hlistmem s |= Fs * haddr GDisk |-> vd /\
+       Inv m s d /\
+       (* cache_get (get Cache m) a = None /\ *)
+       vd |= lin_pred F NoOwner * lin_pred
+                                    (cache_locked tid s (LF * a |-> (v, None))) (Owned tid) /\
+       R tid s0 s
+   | POST d' m' s0' s' r:
+       exists vd',
+         hlistmem s' |= Fs' * haddr GDisk |-> vd' /\
+         Inv m' s' d' /\
+         vd' |= lin_pred F' NoOwner * lin_pred
+                                        (cache_locked tid s (LF * a |-> (v, None))) (Owned tid) /\
+         r = v /\
+         R tid s0' s'
+  }} locked_AsyncRead a.
+Proof.
+Abort.
+
+Definition read {T} a rx : prog Mcontents Scontents T :=
+  tid <- GetTID;
+  c <- Get Cache;
+  match cache_get c a with
+  | Some (Clean v) => rx v
+  | Some (Dirty v) => rx v
+  | None => v <- locked_AsyncRead a;
+      let c' := cache_add c a v in
+      Assgn Cache c';;
+            rx v
+  end.
+
+
+End Cache.
